NumLean/Data/HTuple.lean
@@ -1,3 +1,4 @@
 import NumLean.Data.HTuple.Basic
 import NumLean.Data.HTuple.Ops
 import NumLean.Data.HTuple.Algebra
+import NumLean.Data.HTuple.RangeIterator
